thy/Routing/IpRoute_Parser.thy
@@ -4,28 +4,28 @@ imports Routing_Table
   "../IP_Addresses/IP_Address_Parser"
 keywords "parse_ip_route" :: thy_decl
 begin
-text\<open>This helps to read the output of the \texttt{ip route} command into a @{typ "routing_rule list"}.\<close>
+text\<open>This helps to read the output of the \texttt{ip route} command into a @{typ "32 routing_rule list"}.\<close>
 
-definition empty_rr_hlp :: "32 prefix_match \<Rightarrow> routing_rule" where
+definition empty_rr_hlp :: "32 prefix_match \<Rightarrow> 32 routing_rule" where
   "empty_rr_hlp pm = routing_rule.make pm default_metric (routing_action.make '''' None)"
 
 lemma empty_rr_hlp_alt:
   "empty_rr_hlp pm = \<lparr> routing_match = pm, metric = 0, routing_action = \<lparr>output_iface = [], next_hop = None\<rparr>\<rparr>"
   unfolding empty_rr_hlp_def routing_rule.defs default_metric_def routing_action.defs ..
 
-definition routing_action_next_hop_update :: "32 word \<Rightarrow> routing_rule \<Rightarrow> routing_rule"
+definition routing_action_next_hop_update :: "32 word \<Rightarrow> 32 routing_rule \<Rightarrow> 32 routing_rule"
   where
   "routing_action_next_hop_update h pk = pk\<lparr> routing_action := (routing_action pk)\<lparr> next_hop := Some h\<rparr> \<rparr>"
-lemma "routing_action_next_hop_update h pk = routing_action_update (next_hop_update (\<lambda>_. (Some h))) (pk::routing_rule)"
+lemma "routing_action_next_hop_update h pk = routing_action_update (next_hop_update (\<lambda>_. (Some h))) (pk::32 routing_rule)"
   by(simp add: routing_action_next_hop_update_def)
 
-definition routing_action_oiface_update :: "string \<Rightarrow> routing_rule \<Rightarrow> routing_rule"
+definition routing_action_oiface_update :: "string \<Rightarrow> 32 routing_rule \<Rightarrow> 32 routing_rule"
   where
-  "routing_action_oiface_update h pk = routing_action_update (output_iface_update (\<lambda>_. h)) (pk::routing_rule)"
+  "routing_action_oiface_update h pk = routing_action_update (output_iface_update (\<lambda>_. h)) (pk::32 routing_rule)"
 lemma "routing_action_oiface_update h pk = pk\<lparr> routing_action := (routing_action pk)\<lparr> output_iface :=  h\<rparr> \<rparr>"
   by(simp add: routing_action_oiface_update_def)
 
-definition "sanity_ip_route r \<equiv> correct_routing r \<and> list_all (op \<noteq> '''' \<circ> routing_oiface) r"
+definition "sanity_ip_route (r::32 prefix_routing) \<equiv> correct_routing r \<and> list_all (op \<noteq> '''' \<circ> routing_oiface) r"
 text\<open>The parser ensures that @{const sanity_ip_route} holds for any ruleset that is imported.\<close>
 
 (* Hide all the ugly ml in a file with the right extension *)
@@ -39,7 +39,7 @@ ML\<open>
 \<close>
 
 parse_ip_route "rtbl_parser_test1" = "ip-route-ex"
-lemma  "sanity_ip_route rtbl_parser_test1" by eval
+lemma  "sanity_ip_route rtbl_parser_test1" by eval (* checked by parse_ip_route alread *)
 
 lemma "rtbl_parser_test1 =
   [\<lparr>routing_match = PrefixMatch 0xFFFFFF00 32, metric = 0, routing_action = \<lparr>output_iface = ''tun0'', next_hop = None\<rparr>\<rparr>,
